Translation/Term/Lemmas.lean
@@ -18,16 +18,135 @@ import Surface.Typing
 
 def Surface.TyEnv.translate (G : Core.GlobalEnv) (Δ : Core.KindEnv) (Γ : Surface.TyEnv) : Option (Core.TyEnv) := Γ.mapM (·.translate G Δ )
 
+
+theorem Translation.KindEnv.lift_sound  {Δ : Surface.KindEnv} {Δ' : Core.KindEnv} {K : Surface.Kind} {K'}:
+  Δ.translate = Δ' ->
+  K.translate = K' ->
+  Surface.KindEnv.translate (K::Δ) = K' :: Δ':= by
+intro h1 h2
+rw[Surface.KindEnv.translate, List.map_cons]
+rw[Surface.KindEnv.translate] at h1
+simp [h1, h2]
+
+theorem Translation.TyEnv.kindenv_lift_sound
+  {Δ : Surface.KindEnv} {Δ' : Core.KindEnv}
+  {Γ : Surface.TyEnv} {Γ' : Core.TyEnv}
+  {K : Surface.Kind} {K' : Core.Kind}:
+  Γ.translate G' Δ' = some Γ' ->
+  K.translate = K' ->
+  Surface.KindEnv.translate (K::Δ) = (K'::Δ') ->
+  Surface.TyEnv.translate G' (K'::Δ') (Γ.map (·[+1])) = some (Γ'.map (·[+1]))
+   := by
+intro h1 h2 h3
+unfold Surface.TyEnv.translate;
+sorry
+
+
+theorem Translation.TyEnv.sound {G : Core.GlobalEnv} {Δ : Core.KindEnv} {Γ : Surface.TyEnv} {Γ' : Core.TyEnv} :
+  Γ.translate G Δ = some Γ' ->
+  (∀ (i : Nat) (T : Surface.Ty),
+     (Γ[i]? = some T) -> ∃ T', ((Γ'[i]? = some T') ∧ T.translate G Δ = some T')) := by
+intro h1 i K h2;
+
+sorry
+
+
+theorem Translation.GlobalEnv.sound {G : Surface.GlobalEnv} :
+  ⊢s G ->
+  G.translate = some G' ->
+  (∀ (x : String) (T : Surface.Ty) (Δ : Core.KindEnv),
+    (Surface.lookup_type G x = some T) ->
+    ∃ T' b, (Core.lookup_type G' x = some T' ∧ T.translate G' Δ = some T' ∧ G'&Δ ⊢ T' : .base b)) := by
+intro h1 i K h2; sorry
+
+
+
 theorem Translation.Term.Sound (G : Surface.GlobalEnv) :
   ⊢s G ->
   G&Δ,Γ ⊢s t : T ->
+
+
   G.translate = some G' ->
   Δ.translate = Δ' ->
   Γ.translate G' Δ' = some Γ' ->
 
-  (T.translate G' Δ' = some T' ∧
+  ∃ T' t', (T.translate G' Δ' = some T' ∧
   t.translate G' Δ' Γ' = some t' ∧
   t'.Determined ∧
   G'&Δ',Γ' ⊢ t' : T') := by
+intro wf j h1 h2 h3
+induction j generalizing Δ' Γ' <;> simp at *
+case var Γ x T Δ b h jk =>
+  have lem := Translation.TyEnv.sound h3 x T h
+  rcases lem with ⟨T', h4, h5⟩
+  replace jk := Translation.Ty.sound wf ⟨jk, h1 , h2⟩
+  rcases jk with ⟨K', T', h6, h7, h8⟩
+  have h6' := Translation.Kind.sound_base (b := b);
+  rcases h6' with ⟨b', h6'⟩;
+  rw[h6'] at h6; subst h6
+  rw[h7] at h5; cases h5
+  exists T'
+  constructor
+  · assumption
+  · constructor
+    · unfold Core.Term.Determined; apply Core.VariantMissing.var
+    · apply Core.Typing.var; repeat assumption
+case global x T Δ b Γ h4 j =>
+  have lem := Translation.GlobalEnv.sound wf h1 x T Δ' h4
+  rcases lem with ⟨T', h4, h5, h6, h7⟩
+  exists T'
+  constructor
+  · assumption
+  · constructor
+    unfold Core.Term.Determined; apply Core.VariantMissing.global
+    apply Core.Typing.global;
+    assumption
+    assumption
 
-sorry
+case lam Δ A b1 B b2 Γ t j1 j2 j3 ih =>
+  have lemA := Translation.Ty.sound wf ⟨j1, h1, h2⟩
+  rcases lemA with ⟨aK', A', h4a, h5a, h6a⟩
+  have lemB := Translation.Ty.sound wf ⟨j2, h1, h2⟩
+  rcases lemB with ⟨bK', B', h4b, h5b, h6b⟩
+  have h6' := Translation.Kind.sound_base (b := b1)
+  rcases h6' with ⟨b1', h6'⟩
+  have h6'' := Translation.Kind.sound_base (b := b2)
+  rcases h6'' with ⟨b2', h6''⟩
+  rw[h6'] at h4a; subst h4a; clear h6'
+  rw[h6''] at h4b; subst h4b; clear h6''
+  exists (A' -:> B'); rw[Option.bind_eq_some_iff]
+  constructor
+  · exists A'; constructor; assumption;
+    rw[Option.bind_eq_some_iff]; simp; assumption
+  · have lem : Surface.TyEnv.translate G' Δ' (A :: Γ) = some (A' :: Γ') := by
+      rw [Surface.TyEnv.translate]; unfold Surface.TyEnv.mapM; rw[<-List.mapM'_eq_mapM]
+      simp [bind, instMonadOption, Option.bind_eq_some_iff];
+      constructor; assumption; rw[Surface.TyEnv.translate] at h3; rw[List.mapM'_eq_mapM]
+      apply h3;
+    replace ih := @ih Δ' (A' :: Γ') h2 lem
+    rcases ih with ⟨B', h7, t', h9, h10, h11⟩
+    exists λ[A']t'; rw[Option.bind_eq_some_iff];
+    constructor;
+    · exists A'; constructor; assumption;
+      rw[Option.bind_eq_some_iff]; exists t'
+    · constructor
+      · constructor; assumption
+      · rw[h5b] at h7; cases h7;
+        apply Core.Typing.lam; assumption; assumption
+case lamt Δ K P t Γ j1 j2 ih =>
+  have lem := Translation.Ty.sound wf ⟨j1, h1, h2⟩
+  rcases lem with ⟨K', T', h4, h5, h6⟩
+  simp at h5; rw[Option.bind_eq_some_iff] at h5;
+  rcases h5 with ⟨P', h7, h8⟩
+  cases h8; simp at h4; subst K'
+  exists (∀[K.translate]P')
+  rw[Option.bind_eq_some_iff]
+  constructor
+  · simp; assumption
+  · replace ih := @ih (K.translate :: Δ') (Γ'.map (·[+1]))
+    sorry
+case app =>
+  sorry
+case appt =>
+  sorry
+case mtch => sorry
